Generates a segfault in ugraph

common/theories/uGraph.v
@@ -76,6 +76,75 @@ Qed.
 
 End Push.
 
+Definition levels_of_list (l : list Level.t) : LevelSet.t :=
+  List.fold_right LevelSet.add LevelSet.empty l.
+
+Definition constraints_of_list (l : list UnivConstraint.t) : UnivConstraintSet.t :=
+  List.fold_right UnivConstraintSet.add UnivConstraintSet.empty l.
+
+Import MRMonadNotation.
+
+Declare Scope cstr_scope.
+Delimit Scope cstr_scope with cstr.
+Bind Scope cstr_scope with UnivConstraint.t.
+Notation " x <= y " := (@pair (Universe.t * UnivConstraintType.ConstraintType.t) Universe.t
+  (@pair Universe.t _ x Le) y) : cstr_scope.
+
+Definition of_level (l : Level.t_) : Universe.t := Universe.of_level l.
+Coercion of_level : Level.t_ >-> Universe.t.
+Coercion Universe.of_level : Level.t >-> Universe.t.
+
+Definition test_model : bool :=
+  let la := Level.level "a" in
+  let lb := Level.level "b" in
+  let ls := levels_of_list [la; lb] in
+  let cs := constraints_of_list [(la <= lb)%cstr] in
+  match push_uctx init_model (ls, cs) with
+  | Some m => true
+  | None => false
+  end.
+
+Lemma test_model_spec : test_model = true.
+Proof.
+  rewrite /test_model.
+  set ls := levels_of_list _.
+  set cs := constraints_of_list _.
+  rewrite /push_uctx /push_uctx_clause_1.
+  set m := UnivLoopChecking.declare_levels init_model ls.
+  rewrite /enforce_constraints /enforce_constraints_aux.
+  cbn -[enforce].
+  set m' := {| model := _ |}.
+  unfold enforce.
+  set ef := LoopCheck.enforce m' _.
+  cbn -[LoopCheck.enforce] in ef.
+  unfold to_atoms in ef.
+  cbn -[LoopCheck.enforce] in ef.
+  unfold LoopCheck.enforce in ef.
+  unfold LoopCheck.Impl.Abstract.enforce_clauses in ef.
+  hnf in ef.
+  unfold LoopCheck.Impl.CorrectModel.infer_extension_correct in ef.
+  unfold LoopCheck.Impl.CorrectModel.infer_extension_correct_clause_1 in ef.
+  unfold LoopCheck.Impl.infer_extension in ef.
+  unfold LoopCheck.Impl.infer_model_extension in ef.
+  hnf in ef.
+  set (l := LoopCheck.Impl.I.loop _ _ _ _ _ _) in *.
+  match goal with
+  | [ l := LoopCheck.Impl.I.loop _ _ _ _ _ ?pre |- _ ] =>
+    set (precond := pre) in *
+  end.
+  clearbody precond.
+
+
+  lazy in ef.
+  unfold LoopCheck.Impl.I.loop in ef.
+  hnf in ef.
+  set ()
+  unfold FixWf in ef.
+
+  hnf in ef.
+  Eval compute in test_model.
+
+
 Import UnivLoopChecking.
 
 (** ** Check of consistency ** *)
